\input{../utils/preamble}
\createdgmtitle{9}
%--------------------------------------------------------------------------------
\begin{document}
%--------------------------------------------------------------------------------
\begin{frame}[noframenumbering,plain]
%\thispagestyle{empty}
\titlepage
\end{frame}
%=======
\begin{frame}{Recap of previous lecture}
	Let perturb original data by normal noise $q(\bx_{\sigma} | \bx) = \cN(\bx, \sigma^2 \cdot \bI)$
	\vspace{-0.3cm}
	\[
	q(\bx_{\sigma}) = \int q(\bx_{\sigma} | \bx) \pi(\bx) d\bx.
	\]
	\vspace{-0.6cm} \\
	Then the solution of 
	\vspace{-0.2cm}
	\[
	\frac{1}{2} \bbE_{q(\bx_{\sigma})}\bigl\| \bs_{\btheta, \sigma}(\bx_{\sigma}) - \nabla_{\bx_{\sigma}} \log q(\bx_{\sigma}) \bigr\|^2_2 \rightarrow \min_{\btheta}
	\]
	\vspace{-0.5cm} \\
	satisfies $\bs_{\btheta, \sigma}(\bx_{\sigma}) \approx \bs_{\btheta, 0}(\bx_0) = \bs_{\btheta}(\bx)$ if $\sigma$ is small enough.
	\begin{block}{Theorem (denoising score matching)}
		\vspace{-0.8cm}
		\begin{multline*}
			\bbE_{q(\bx_{\sigma})}\bigl\| \bs_{\btheta, \sigma}(\bx_{\sigma}) - \nabla_{\bx_{\sigma}} \log q(\bx_{\sigma}) \bigr\|^2_2 = \\ = \bbE_{\pi(\bx)} \bbE_{q(\bx_{\sigma} | \bx)}\bigl\| \bs_{\btheta, \sigma}(\bx_{\sigma}) - \nabla_{\bx_{\sigma}} \log q(\bx_{\sigma} | \bx) \bigr\|^2_2 + \text{const}(\btheta)
		\end{multline*}
		\vspace{-0.7cm}
	\end{block}
	Here $\nabla_{\bx_{\sigma}} \log q(\bx_{\sigma} | \bx) = - \frac{\bx_{\sigma} - \bx}{\sigma^2} = - \frac{\bepsilon}{\sigma}$.
	\begin{itemize}
		\item We do not need to compute $\nabla_{\bx_{\sigma}} \log q(\bx_{\sigma})$ at the RHS.
		\item $\bs_{\btheta, \sigma}(\bx_{\sigma})$ tries to \textbf{denoise} a corrupted sample.
	\end{itemize}
	\myfootnotewithlink{http://www.iro.umontreal.ca/~vincentp/Publications/smdae_techreport.pdf}{Vincent P. A Connection Between Score Matching and Denoising Autoencoders, 2010}
\end{frame}
%=======
\begin{frame}{Recap of previous lecture}
	\begin{block}{Noise conditioned score network}
		\begin{itemize}
			\item Define the sequence of noise levels: $\sigma_1 < \sigma_2 < \dots < \sigma_T$.
			\item Train denoised score function $\bs_{\btheta, \sigma_t}(\bx_t)$ for each noise level:
			\vspace{-0.3cm}
			\[
				\sum_{t=1}^T {\color{violet}\sigma_t^2} \cdot \bbE_{\pi(\bx)} \bbE_{q(\bx_t | \bx)}\bigl\| \bs_{\btheta, \sigma_t}(\bx_t) - \nabla_{\bx_t} \log q(\bx_t | \bx) \bigr\|^2_2 \rightarrow \min_{\btheta}
			\]
			\vspace{-0.5cm}
			\item Sample from \textbf{annealed} Langevin dynamics (for $t=1, \dots, T$).
		\end{itemize}
	\end{block}
	\begin{figure}
		\includegraphics[width=0.55\linewidth]{figs/multi_scale}
	\end{figure}
	\begin{figure}
		\includegraphics[width=\linewidth]{figs/duoduo}
	\end{figure}
	\myfootnotewithlink{https://arxiv.org/abs/1907.05600}{Song Y. et al. Generative Modeling by Estimating Gradients of the Data Distribution, 2019}
\end{frame}
%=======
\begin{frame}{Recap of previous lecture}
	\begin{block}{NCSN training}
		\begin{enumerate}
			\item Get the sample $\bx_0 \sim \pi(\bx)$.
			\item Sample noise level $t \sim U\{1, T\}$ and the noise $\bepsilon \sim \cN(0, \bI)$.
			\item Get noisy image $\bx_t = \bx_0 + \sigma_t \cdot \bepsilon$.
			\item Compute loss $ \cL = \sigma_t^2 \cdot \| \bs_{\btheta, \sigma_t}(\bx_t) + \frac{\bepsilon}{\sigma_t} \|^2 $.
		\end{enumerate}
	\end{block}
	\begin{block}{NCSN sampling (annealed Langevin dynamics)}
		\begin{itemize}
			\item Sample $\bx_0 \sim \cN(0, \sigma_T^2 \cdot \bI) \approx q(\bx_T)$.
			\item Apply $L$ steps of Langevin dynamic
			\vspace{-0.2cm}
			\[
				\bx_l = \bx_{l-1} + \frac{\eta_t}{2} \cdot \bs_{\btheta, \sigma_t}(\bx_{l - 1}) + \sqrt{\eta_t} \cdot \bepsilon_l.
			\] 
			\vspace{-0.5cm}
			\item Update $\bx_0 := \bx_L$ and choose the next $\sigma_t$.
		\end{itemize}
	\end{block}
	\myfootnotewithlink{https://arxiv.org/abs/2006.09011}{Song Y. et al. Improved Techniques for Training Score-Based Generative Models, 2020}
\end{frame}
%=======
\begin{frame}{Recap of previous lecture}
	\begin{block}{Forward Gaussian diffusion process}
		Let $\bx_0 = \bx \sim \pi(\bx)$, $\beta_t \ll 1$, $\alpha_t = 1 - \beta_t$ and $\bar{\alpha}_t = \prod_{s=1}^t \alpha_s$. 
		\begin{align*}
			\bx_t &= \sqrt{1 - \beta_t} \cdot \bx_{t - 1} + \sqrt{\beta_t} \cdot \bepsilon, \quad \text{where }\bepsilon \sim \cN(0, \bI); \\
			\bx_t &= \sqrt{\bar{\alpha}_t} \cdot \bx_{0} + \sqrt{1 - \bar{\alpha}_t} \cdot \bepsilon, \quad \text{where } \bepsilon \sim \cN(0, \bI).
		\end{align*}
		\vspace{-0.6cm}
		\begin{align*}
			q(\bx_t | \bx_{t-1}) &= \cN(\sqrt{1 - \beta_t} \cdot \bx_{t-1}, \beta_t \cdot \bI); \\
			q(\bx_t | \bx_0) &= \cN(\sqrt{\bar{\alpha}_t} \cdot \bx_0, (1 - \bar{\alpha}_t) \cdot \bI).
		\end{align*}
		\vspace{-0.6cm}
	\end{block}
	\begin{figure}
		\includegraphics[width=0.8\linewidth]{figs/conditional_diffusion}
	\end{figure}
	\myfootnotewithlink{https://arxiv.org/abs/2403.18103}{Chan S. Tutorial on Diffusion Models for Imaging and Vision, 2024}
\end{frame}
%=======
\begin{frame}{Recap of previous lecture}
	\textbf{Diffusion} refers to the flow of particles from high-density regions towards low-density regions.
	\vspace{-0.2cm}
	\begin{figure}
		\includegraphics[width=0.5\linewidth]{figs/diffusion_over_time}
	\end{figure}
	\vspace{-0.6cm}
	\begin{enumerate}
		\item $\bx_0 = \bx \sim \pi(\bx)$;
		\item $\bx_t = \sqrt{1 - \beta_t} \cdot \bx_{t - 1} + \sqrt{\beta_t} \cdot \bepsilon$, where $\bepsilon \sim \cN(0, \bI)$, $t \geq 1$;
		\item $\bx_T \sim p_{\infty}(\bx) = \cN(0, \bI)$, where $T \gg 1$.
	\end{enumerate}
	If we are able to invert this process, we will get the way to sample $\bx \sim \pi(\bx)$ using noise samples $p_{\infty}(\bx) = \cN(0, \mathbf{I})$. \\ 
	Now our goal is to revert this process.
	\myfootnotewithlink{https://ayandas.me/blog-tut/2021/12/04/diffusion-prob-models.html}{Das A. An introduction to Diffusion Probabilistic Models, blog post, 2021}
\end{frame}
%=======
\begin{frame}{Outline}
	\tableofcontents
\end{frame}
%=======
\section{Denoising Diffusion Probabilistic Model (DDPM)}
%=======
\subsection{Gaussian diffusion model as VAE}
%=======
\begin{frame}{Gaussian diffusion model as VAE}
	Let treat $\bz = (\bx_1, \dots, \bx_T)$ as a latent variable (\textbf{note:} each $\bx_t$ has the same size) and $\bx = \bx_0$ as observed samples. 
	\begin{block}{Latent Variable Model}
		\vspace{-0.3cm}
		\[
			p(\bx, \bz | \btheta) = p(\bx | \bz, \btheta) p(\bz | \btheta)
		\]	
		\vspace{-0.7cm}
	\end{block}
	\begin{figure}
		\includegraphics[width=0.8\linewidth]{figs/diffusion_pgm_forward}
	\end{figure}
	\vspace{-0.3cm}
	\begin{block}{Forward diffusion}
		\begin{itemize}
			\item Variational posterior distribution (encoder)
			\vspace{-0.3cm}
			\[
				q(\bz | \bx) = q(\bx_1, \dots, \bx_T | \bx_0) = \prod_{t = 1}^T q(\bx_t | \bx_{t - 1}).
			\]
			\item \textbf{Note:} there is no learnable parameters.
		\end{itemize}
		\vspace{-0.5cm}
	\end{block}
	\myfootnotewithlink{https://ayandas.me/blog-tut/2021/12/04/diffusion-prob-models.html}{Das A. An introduction to Diffusion Probabilistic Models, blog post, 2021}
\end{frame}
%=======
\begin{frame}{Gaussian diffusion model as VAE}
	\vspace{-0.3cm}
	\[
		p(\bx, \bz | \btheta) = p(\bx | \bz, \btheta) p(\bz | \btheta)
	\]	
	\vspace{-0.3cm}
	\begin{figure}
		\includegraphics[width=0.8\linewidth]{figs/diffusion_pgm_reverse}
	\end{figure}
	\vspace{-0.2cm}
	\begin{block}{Reverse diffusion}
		\begin{itemize}
			\item Generative distribution (decoder)
			\[
				p(\bx | \bz, \btheta) = p(\bx_0 | \bx_1, \btheta).
			\]
			\item Prior distribution
			\vspace{-0.3cm}
			\[
				p(\bz | \btheta) = p(\bx_1, \dots, \bx_T | \btheta) = \prod_{t=2}^T p(\bx_{t - 1} | \bx_t, \btheta)  \cdot p(\bx_T).
			\]
		\end{itemize}
		\textbf{Note:} this differs from the vanilla VAE with the complex decoder $p(\bx | \bz, \btheta)$ and the standard normal prior $p(\bz)$.
	\end{block}
	\myfootnotewithlink{https://ayandas.me/blog-tut/2021/12/04/diffusion-prob-models.html}{Das A. An introduction to Diffusion Probabilistic Models, blog post, 2021}
\end{frame}
%=======
\subsection{ELBO derivation}
%=======
\begin{frame}{ELBO for Gaussian diffusion model}
	\begin{block}{Standard ELBO}
		\vspace{-0.3cm}
		\[
			\log p(\bx | \btheta) \geq \bbE_{q({\color{teal}\bz} | \bx)} \log \frac{p(\bx, {\color{teal}\bz} | \btheta)}{q({\color{teal}\bz} | \bx)} = \cL_{\bphi, \btheta}(\bx) \rightarrow \max_{q, \btheta}
		\]
		\vspace{-0.5cm}
	\end{block}
	\begin{block}{Derivation}
		\vspace{-0.5cm}
		\begin{align*}
			\cL_{\bphi, \btheta}(\bx) &= \bbE_{q({\color{teal}\bx_{1:T}} | \bx_0)} \log \frac{p(\bx_0, {\color{teal}\bx_{1:T}} | \btheta)}{q({\color{teal}\bx_{1:T}} | \bx_0)} \\
			& = \bbE_{q(\bx_{1:T} | \bx_0)} \log \frac{p(\bx_T) \prod_{t=1}^T p(\bx_{t-1} | \bx_t, \btheta) }{\prod_{t=1}^T {\color{violet}q(\bx_t | \bx_{t-1})}}
		\end{align*}
		\vspace{-0.3cm}
		\begin{itemize}
			\item Let try to decompose the ELBO to separate KL divergences.
			\item We have to swap the distribution $q(\bx_t | \bx_{t - 1})$ to $q(\bx_{t - 1} | \bx_t)$ in the denominator.
			\item Let add conditioning on $\bx_0$ to make reverse distribution $q(\bx_{t - 1} | \bx_t)$ tractable.
		\end{itemize}
	\end{block}
	
	\myfootnotewithlink{https://arxiv.org/abs/2006.11239}{Ho J. Denoising Diffusion Probabilistic Models, 2020}
\end{frame}
%=======
\begin{frame}{ELBO for Gaussian diffusion model}
	\[
		 {\color{teal}q(\bx_t | \bx_{t-1}, \bx_0)}  = \frac{q(\bx_{t-1}|\bx_t, \bx_0)q(\bx_{t} | \bx_0)}{q(\bx_{t-1}| \bx_0)}
	\]
	\vspace{-0.3cm}
	\begin{block}{Derivation (continued)}
		\vspace{-0.6cm}
		{\small
		\begin{align*}
			\cL_{\bphi, \btheta}(\bx) & = \bbE_{q(\bx_{1:T} | \bx_0)} \log \frac{p(\bx_T) \prod_{t=1}^T p(\bx_{t-1} | \bx_t, \btheta) }{\prod_{t=1}^T {\color{violet}q(\bx_t | \bx_{t-1})}}  \\ 
			& = \bbE_{q(\bx_{1:T} | \bx_0)} \log \frac{p(\bx_T) \prod_{t=1}^T p(\bx_{t-1} | \bx_t, \btheta) }{\prod_{t=1}^T q(\bx_t | \bx_{t-1}, {\color{olive}\bx_0})}  \\ 
			& = \bbE_{q(\bx_{1:T} | \bx_0)} \log \frac{p(\bx_T) p(\bx_0 | \bx_1, \btheta) \prod_{t=2}^T p(\bx_{t-1} | \bx_t, \btheta) }{q(\bx_1 | \bx_0)\prod_{t=2}^T {\color{teal}q(\bx_t | \bx_{t-1}, \bx_0)}} \\
			& = \bbE_{q(\bx_{1:T} | \bx_0)} \log \frac{p(\bx_T) p(\bx_0 | \bx_1, \btheta) \prod_{t=2}^T p(\bx_{t-1} | \bx_t, \btheta) }{{\color{violet}q(\bx_1 | \bx_0)}\prod_{t=2}^T \frac{q(\bx_{t-1}|\bx_t, \bx_0) {\color{violet}q(\bx_{t} | \bx_0)}}{{\color{violet}q(\bx_{t-1}| \bx_0)}}} \\
			& = \bbE_{q(\bx_{1:T} | \bx_0)} \log \frac{{\color{violet}p(\bx_T)} {\color{olive}p(\bx_0 | \bx_1, \btheta)} \prod_{t=2}^T p(\bx_{t-1} | \bx_t, \btheta) }{{\color{violet}q(\bx_T | \bx_0)}\prod_{t=2}^T q(\bx_{t-1}|\bx_t, \bx_0)} 
		\end{align*}}
	\end{block}
	
	\myfootnotewithlink{https://arxiv.org/abs/2006.11239}{Ho J. Denoising Diffusion Probabilistic Models, 2020}
\end{frame}
%=======
\begin{frame}{ELBO for Gaussian diffusion model}
	\begin{block}{Derivation (continued)}
		\vspace{-0.7cm}
		{\small
		\begin{multline*}
			\cL_{\bphi, \btheta}(\bx) = \bbE_{q(\bx_{1:T} | \bx_0)} \log \frac{{\color{violet}p(\bx_T)} {\color{olive}p(\bx_0 | \bx_1, \btheta)} \prod_{t=2}^T p(\bx_{t-1} | \bx_t, \btheta) }{{\color{violet}q(\bx_T | \bx_0)}\prod_{t=2}^T q(\bx_{t-1}|\bx_t, \bx_0)}  = \\
			= \bbE_{{\color{teal}q(\bx_{1:T} | \bx_0)}} \biggl[ \log {\color{olive}p(\bx_0 | \bx_1, \btheta)} + \log {\color{violet}\frac{p(\bx_T)}{q(\bx_T | \bx_0)}} + \sum_{t=2}^T \log \left( \frac{p(\bx_{t-1} | \bx_t, \btheta)}{q(\bx_{t-1}|\bx_{t}, \bx_0)}\right) \biggr] = \\
			 = \bbE_{{\color{teal}q(\bx_1 | \bx_0)}} \log p(\bx_0 | \bx_1, \btheta) + \bbE_{{\color{teal}q(\bx_T | \bx_0)}} \log \frac{p(\bx_T)}{q(\bx_T | \bx_0)} + \\
			  + \sum_{t=2}^T \bbE_{{\color{teal}q(\bx_{t-1}, \bx_t | \bx_0)}} \log \left( \frac{p(\bx_{t-1} | \bx_t, \btheta)}{q(\bx_{t-1}|\bx_{t}, \bx_0)}\right) = \\
			  = \bbE_{q(\bx_1 | \bx_0)} \log p(\bx_0 | \bx_1, \btheta) - KL\bigl(q(\bx_T | \bx_0) || p(\bx_T)\bigr) - \\
			  			- \sum_{t=2}^T \underbrace{ \bbE_{q(\bx_t | \bx_0)} KL \bigl(q(\bx_{t-1} | \bx_t, \bx_0) || p(\bx_{t - 1} | \bx_t, \btheta )\bigr)}_{\cL_t}
		\end{multline*}
		}
		\vspace{-0.3cm}
	\end{block}
	\myfootnotewithlink{https://arxiv.org/abs/2006.11239}{Ho J. Denoising Diffusion Probabilistic Models, 2020}
\end{frame}
%=======
\begin{frame}{ELBO for Gaussian diffusion model}
		\vspace{-0.5cm}
		\begin{multline*}
			\cL_{\bphi, \btheta}(\bx) =  {\color{olive}\bbE_{q(\bx_1 | \bx_0)} \log p(\bx_0 | \bx_1, \btheta)} - {\color{violet}KL\bigl(q(\bx_T | \bx_0) || p(\bx_T)\bigr)} - \\
			- {\color{teal}\sum_{t=2}^T \underbrace{ \bbE_{q(\bx_t | \bx_0)} KL \bigl(q(\bx_{t-1} | \bx_t, \bx_0) || p(\bx_{t - 1} | \bx_t, \btheta )\bigr)}_{\cL_t}}
		\end{multline*}
		\vspace{-0.5cm}
	\begin{itemize}
		\item {\color{olive}First term} is a decoder distribution
		\[
			\log p(\bx_0 | \bx_1, \btheta) = \log \cN \bigl(\bx_0 | \bmu_{\btheta, t}(\bx_1), \bsigma_{\btheta, t}^2(\bx_1)\bigr),
		\] 
		with $\bx_1 \sim q(\bx_1 | \bx_0)$.
		\item {\color{violet}Second term} is constant 
		\begin{itemize}
			\item $p(\bx_T) = \cN(0, \bI)$;
			\item $q(\bx_T | \bx_0) = \cN(\sqrt{\bar{\alpha}_T} \cdot \bx_0, (1 - \bar{\alpha}_T) \cdot \bI)$.
		\end{itemize}
		\item {\color{teal}Third term} makes the main contribution to the ELBO.
	\end{itemize}
	\myfootnotewithlink{https://arxiv.org/abs/2006.11239}{Ho J. Denoising Diffusion Probabilistic Models, 2020}
\end{frame}
%=======
\begin{frame}{ELBO for Gaussian diffusion model}
	\begin{figure}
		\includegraphics[width=\linewidth]{figs/diffusion_objective}
	\end{figure}
	\[
		\cL_t = \bbE_{q(\bx_t | \bx_0)} KL \bigl(q(\bx_{t-1} | \bx_t, \bx_0) || p(\bx_{t - 1} | \bx_t, \btheta )\bigr)
	\]
	\begin{align*}
		q(\bx_{t-1} | \bx_t, \bx_0) &= \cN(\bx_{t-1} | \tilde{\bmu}_t(\bx_t, \bx_0), \tilde{\beta}_t \bI), \\
		p(\bx_{t - 1} | \bx_t, \btheta) &= \cN \bigl(\bx_{t - 1} | \bmu_{\btheta, t}(\bx_t), \bsigma_{\btheta, t}^2(\bx_t)\bigr)
	\end{align*}
	\myfootnotewithlink{https://arxiv.org/abs/2208.11970}{Luo C. Understanding Diffusion Models: A Unified Perspective, 2022}
\end{frame}
%=======
\begin{frame}{ELBO for Gaussian diffusion model}
	\vspace{-0.3cm}
	\[
		\cL_t = \bbE_{q(\bx_t | \bx_0)} KL \bigl(q(\bx_{t-1} | \bx_t, \bx_0) || p(\bx_{t - 1} | \bx_t, \btheta )\bigr)
	\]
	\vspace{-0.4cm}
	\begin{align*}
		q(\bx_{t-1} | \bx_t, \bx_0) &= \cN(\bx_{t-1} | \tilde{\bmu}_t(\bx_t, \bx_0), \tilde{\beta}_t \bI), \\
		p(\bx_{t - 1} | \bx_t, \btheta) &= \cN \bigl(\bx_{t - 1} | \bmu_{\btheta, t}(\bx_t), {\color{violet}\bsigma_{\btheta, t}^2(\bx_t)}\bigr)
	\end{align*}
	Let assume
	\[
		{\color{violet}\bsigma_{\btheta, t}^2(\bx_t) = \tilde{\beta}_t \bI} \quad \Rightarrow \quad p(\bx_{t - 1} | \bx_t, \btheta) = \cN \bigl(\bx_{t - 1} | \bmu_{\btheta, t}(\bx_t), {\color{violet}\tilde{\beta}_t \bI} \bigr).
	\]
	Theoretically optimal $\bsigma_{\btheta, t}^2(\bx_t)$ lies in the range $[\tilde{\beta}_t, \beta_t]$:
	\begin{itemize}
		\item $\beta_t$ is optimal for $\bx_0 \sim \cN(0, \bI)$;
		\item $\tilde{\beta}_t$ is optimal for $\bx_0 \sim \delta(\bx_0 - \bx^*)$.
	\end{itemize}
	\begin{align*}
		\cL_t &= \bbE_{q(\bx_t | \bx_0)} KL\Bigl(\cN\bigl(\tilde{\bmu}_t(\bx_t, \bx_0), \tilde{\beta}_t \bI \bigr) || \cN\bigl(\bmu_{\btheta, t}(\bx_t), \tilde{\beta}_t \bI\bigr)\Bigr) \\ 
		&= \bbE_{q(\bx_t | \bx_0)} \left[\frac{1}{2\tilde{\beta}_t} \bigl\| \tilde{\bmu}_t(\bx_t, \bx_0) - \bmu_{\btheta, t}(\bx_t) \bigr\|^2  \right]
	\end{align*}
	
	\myfootnotewithlink{https://arxiv.org/abs/2006.11239}{Ho J. Denoising Diffusion Probabilistic Models, 2020}
\end{frame}
%=======
\begin{frame}{ELBO for Gaussian diffusion model}
	\begin{block}{Training}
		\begin{enumerate}
			\item Get the sample $\bx_0 \sim \pi(\bx)$.
			\item Get noisy image $\bx_t = \sqrt{\bar{\alpha}_t} \cdot \bx_0 + \sqrt{1 - \bar{\alpha}_t} \cdot \bepsilon$, where $\bepsilon \sim \cN(0, \bI)$.
			\item Compute ELBO 
			\vspace{-0.3cm}
			\begin{multline*}
				\cL_{\bphi, \btheta}(\bx) =  {\color{olive}\bbE_{q(\bx_1 | \bx_0)} \log p(\bx_0 | \bx_1, \btheta)} - {\color{violet}KL\bigl(q(\bx_T | \bx_0) || p(\bx_T)\bigr)} - \\
				- {\color{teal}\sum_{t=2}^T \underbrace{ \bbE_{q(\bx_t | \bx_0)} \left[\frac{1}{2\tilde{\beta}_t} \bigl\| \tilde{\bmu}_t(\bx_t, \bx_0) - \bmu_{\btheta, t}(\bx_t) \bigr\|^2  \right]}_{\cL_t}}
			\end{multline*}
			\vspace{-0.7cm}
		\end{enumerate}
	\end{block}
	\begin{block}{Sampling}
		\begin{enumerate}
			\item Sample $\bx_T \sim \cN(0, \bI)$.
			\item Get denoised image $\bx_{t - 1} = \bmu_{\btheta, t}(\bx_t) +  \sqrt{\tilde{\beta}_t} \cdot \bepsilon$, where $\bepsilon \sim \cN(0, \bI)$.
		\end{enumerate}
	\end{block}
	
	\myfootnotewithlink{https://arxiv.org/abs/2006.11239}{Ho J. Denoising Diffusion Probabilistic Models, 2020}
\end{frame}
%=======
\begin{frame}{Summary}
	\begin{itemize}
		\item DDPM approximates the reverse process using Normal assumption.		
		\vfill
		\item One could treat DDPM as VAE model with hierarchical latent variables.
		\vfill
		\item ELBO of DDPM could be represented as a sum of large number of the KL terms.
	\end{itemize}
\end{frame}
%=======
\end{document} 